src/high/post_crash_modality.v
@@ -19,37 +19,37 @@ Notation base_post_crash := post_crash_modality.post_crash.
 
 (* The three implications for the things stored for a protocolt. *)
 Definition post_crash_pred_impl `{nvmFixedG Σ}
-           (nD nD' : nvmDeltaG Σ) : iProp Σ :=
-  □ ∀ ST (_ : EqDecision ST) (_ : Countable ST) ℓ (ϕ : ST → val → nvmDeltaG Σ → dProp Σ),
+           (nD nD' : nvmDeltaG) : iProp Σ :=
+  □ ∀ ST (_ : EqDecision ST) (_ : Countable ST) ℓ (ϕ : ST → val → nvmDeltaG → dProp Σ),
     know_pred (hGD := nD) ℓ ϕ -∗
     or_lost_post_crash_no_t ℓ (▷ know_pred (hGD := nD') ℓ ϕ).
 
 Definition post_crash_preorder_impl `{nvmFixedG Σ}
-           (nD nD' : nvmDeltaG Σ) : iProp Σ :=
+           (nD nD' : nvmDeltaG) : iProp Σ :=
   □ ∀ ST (_ : EqDecision ST) (_ : Countable ST) (_ : AbstractState ST) ℓ,
     know_preorder_loc (nD := nD) ℓ (abs_state_relation (ST := ST)) -∗
     (or_lost_post_crash_no_t ℓ
       (know_preorder_loc (nD := nD') ℓ (abs_state_relation (ST := ST)))).
 
 Definition post_crash_bumper_impl `{nvmFixedG Σ}
-           (nD nD' : nvmDeltaG Σ) : iProp Σ :=
+           (nD nD' : nvmDeltaG) : iProp Σ :=
   □ ∀ ST (_ : EqDecision ST) (_ : Countable ST) (_ : AbstractState ST)
       ℓ (bumper : ST → ST),
     know_bumper (nD := nD) ℓ bumper -∗
     or_lost_post_crash_no_t ℓ (know_bumper (nD := nD') ℓ bumper).
 
 Definition post_crash_at_loc_impl `{nvmFixedG Σ}
-           (nD nD' : nvmDeltaG Σ) : iProp Σ :=
+           (nD nD' : nvmDeltaG) : iProp Σ :=
   □ ∀ ℓ, is_at_loc (nD := nD) ℓ -∗
     or_lost_post_crash_no_t ℓ (is_at_loc (nD := nD') ℓ).
 
 Definition post_crash_na_loc_impl `{nvmFixedG Σ}
-           (nD nD' : nvmDeltaG Σ) : iProp Σ :=
+           (nD nD' : nvmDeltaG) : iProp Σ :=
   □ ∀ ℓ, is_na_loc (nD := nD) ℓ -∗
     or_lost_post_crash_no_t ℓ (is_na_loc (nD := nD') ℓ).
 
 Definition map_map_phys_history_impl `{nvmFixedG Σ}
-           (nD nD' : nvmDeltaG Σ) : iProp Σ :=
+           (nD nD' : nvmDeltaG) : iProp Σ :=
   □ ∀ ℓ tStore msg,
     know_phys_hist_msg (nD := nD) ℓ tStore msg -∗
       or_lost_post_crash_no_t ℓ (
@@ -57,19 +57,19 @@ Definition map_map_phys_history_impl `{nvmFixedG Σ}
       ).
 
 Definition post_crash_na_view_map `{nvmFixedG Σ}
-           (na_views : gmap loc view) (nD nD' : nvmDeltaG Σ) : iProp Σ :=
+           (na_views : gmap loc view) (nD nD' : nvmDeltaG) : iProp Σ :=
   (∀ ℓ q SV, know_na_view (nD := nD) ℓ q SV -∗ ⌜ na_views !! ℓ = Some SV ⌝) ∗
   [∗ map] ℓ ↦ SV ∈ na_views,
     soft_disj
       (λ q, know_na_view (nD := nD) ℓ q SV)
       (λ q, or_lost_post_crash_no_t ℓ (know_na_view (nD := nD') ℓ q ∅)).
 
-Instance know_na_view_post_crash_fractional `{nvmFixedG Σ, nvmDeltaG Σ} ℓ :
+Instance know_na_view_post_crash_fractional `{nvmFixedG Σ, nvmDeltaG} ℓ :
   Fractional (λ q0 : Qp, or_lost_post_crash_no_t ℓ (know_na_view ℓ q0 ∅)).
 Proof. apply or_lost_post_crash_fractional. apply _. Qed.
 
 Definition know_history_post_crash `{nvmFixedG Σ}
-           (hG : nvmDeltaG Σ) ℓ q bumper (hist : gmap time positive) : iProp Σ :=
+           (hG : nvmDeltaG) ℓ q bumper (hist : gmap time positive) : iProp Σ :=
   or_lost_post_crash ℓ (λ t,
     ∃ sOld sNew,
       ⌜ hist !! t = Some sOld ⌝ ∗
@@ -91,7 +91,7 @@ Proof.
 Qed.
 
 Definition post_crash_frag_history_impl `{hG : nvmFixedG Σ}
-           (nD nD' : nvmDeltaG Σ) : iProp Σ :=
+           (nD nD' : nvmDeltaG) : iProp Σ :=
   □ ∀ ST (_ : EqDecision ST) (_ : Countable ST) (_ : AbstractState ST)
     ℓ (t : nat) (s : ST) (bumper : ST → ST),
       know_preorder_loc (nD := nD) ℓ (abs_state_relation (ST := ST)) -∗
@@ -109,7 +109,7 @@ into a version valid after the crash. *)
 Definition post_crash_full_history_map `{nvmFixedG Σ}
            (hh : gmap loc (gmap time positive))
            (bb : gmap loc (positive → option positive))
-           (nD nD' : nvmDeltaG Σ) : iProp Σ :=
+           (nD nD' : nvmDeltaG) : iProp Σ :=
   (* Used to conclude that the locations owned are included in the heap in question. *)
   (∀ ℓ q hist,
      know_full_encoded_history_loc (nD := nD) ℓ q hist -∗ ⌜hh !! ℓ = Some hist⌝) ∗
@@ -123,7 +123,7 @@ Definition post_crash_full_history_map `{nvmFixedG Σ}
       (λ q, know_history_post_crash nD' ℓ q bumper hist).
 
 Definition post_crash_resource_persistent `{nvmFixedG Σ}
-           (nD nD' : nvmDeltaG Σ) : iProp Σ :=
+           (nD nD' : nvmDeltaG) : iProp Σ :=
   "#post_crash_frag_history_impl" ∷ post_crash_frag_history_impl nD nD' ∗
   "#post_crash_preorder_impl" ∷ post_crash_preorder_impl nD nD' ∗
   "#post_crash_pred_impl" ∷ post_crash_pred_impl nD nD' ∗
@@ -135,22 +135,22 @@ Definition post_crash_resource_persistent `{nvmFixedG Σ}
 Definition post_crash_resource_ephmeral `{nvmFixedG Σ}
            (hh : gmap loc (gmap time positive))
            (bb : gmap loc (positive → option positive))
-           (na_views : gmap loc view) (nD nD' : nvmDeltaG Σ) : iProp Σ :=
+           (na_views : gmap loc view) (nD nD' : nvmDeltaG) : iProp Σ :=
   "post_crash_na_view_map" ∷ post_crash_na_view_map na_views nD nD' ∗
   "post_crash_full_history_map" ∷ post_crash_full_history_map hh bb nD nD'.
 
 Definition post_crash_resource `{nvmFixedG Σ}
            (hh : gmap loc (gmap time positive)) bb
-           (na_views : gmap loc view) (nD nD' : nvmDeltaG Σ) : iProp Σ :=
+           (na_views : gmap loc view) (nD nD' : nvmDeltaG) : iProp Σ :=
   post_crash_resource_persistent nD nD' ∗
   post_crash_resource_ephmeral hh bb na_views nD nD'.
 
-Program Definition post_crash `{nvmFixedG Σ, nD : nvmDeltaG Σ}
-        (P : nvmDeltaG Σ → dProp Σ) : dProp Σ :=
+Program Definition post_crash `{nvmFixedG Σ, nD : nvmDeltaG}
+        (P : nvmDeltaG → dProp Σ) : dProp Σ :=
   MonPred (λ _TV,
     ∀ (hhGD' : nvmHighDeltaG) hh bb na_views,
       base_post_crash (λ nD',
-        let nD' := NvmDeltaG _ nD' hhGD'
+        let nD' := NvmDeltaG nD' hhGD'
         in (post_crash_resource hh bb na_views nD nD') -∗
           ▷ P nD' (∅, ∅, ∅) ∗
           (post_crash_resource_ephmeral hh bb na_views nD nD')))%I
@@ -163,7 +163,7 @@ Notation "'<PC>' g , P" := (post_crash (λ g, P))
 Ltac iIntrosPostCrash := iIntros (hG' hh bb na_views).
 
 Section post_crash_prop.
-  Context `{nvmFixedG Σ, nD: nvmDeltaG Σ}.
+  Context `{nvmFixedG Σ, nD: nvmDeltaG}.
 
   Implicit Types Φ : thread_val → iProp Σ.
   Implicit Types efs : list thread_state.
@@ -267,7 +267,7 @@ Section post_crash_prop.
 End post_crash_prop.
 
 Section post_crash_interact.
-  Context `{nvmFixedG Σ, nD: nvmDeltaG Σ}.
+  Context `{nvmFixedG Σ, nD: nvmDeltaG}.
 
   Context `{AbstractState ST}.
 
@@ -379,7 +379,7 @@ Section post_crash_interact.
     iDestruct 1 as (?) "(% & ? & ? & ?)". iExists _. iFrame. done.
   Qed.
 
-  Lemma post_crash_know_pred `{Countable ST'} ℓ (ϕ : ST' → val → nvmDeltaG Σ → dProp Σ) :
+  Lemma post_crash_know_pred `{Countable ST'} ℓ (ϕ : ST' → val → nvmDeltaG → dProp Σ) :
     ⎡ know_pred ℓ ϕ ⎤ -∗ <PC> _, if_rec ℓ (⎡ know_pred ℓ ϕ ⎤).
   Proof.
     iStartProof (iProp _). iIntros (TV') "HP".
@@ -489,14 +489,14 @@ Section post_crash_interact.
 
 End post_crash_interact.
 
-Class IntoCrash {Σ} `{nvmFixedG Σ, nvmDeltaG Σ}
-      (P : dProp Σ) (Q : nvmDeltaG Σ → dProp Σ) :=
+Class IntoCrash {Σ} `{nvmFixedG Σ, nvmDeltaG}
+      (P : dProp Σ) (Q : nvmDeltaG → dProp Σ) :=
   into_crash : P -∗ post_crash (Σ := Σ) (λ nD', Q nD').
 
 Arguments IntoCrash {_} {_} {_} _%I _%I.
 
 Section IntoCrash.
-  Context `{nvmFixedG Σ, nvmDeltaG Σ}.
+  Context `{nvmFixedG Σ, nvmDeltaG}.
 
   (* Arguments IntoCrash {_} {_} {_} _%I hi%I. *)
 
@@ -622,7 +622,7 @@ Ltac iCrash :=
   let H := iFresh in iIntros H; iNamed H.
 
 Section post_crash_derived.
-  Context `{nvmFixedG Σ, nvmDeltaG Σ}.
+  Context `{nvmFixedG Σ, nvmDeltaG}.
 
   Context `{AbstractState ST}.
 
@@ -659,23 +659,23 @@ Section post_crash_derived.
 
 End post_crash_derived.
 
-(* Definition post_crash_flush `{nvmFixedG Σ, nvmDeltaG Σ} *)
-(*         (P : nvmDeltaG Σ → dProp Σ) : dProp Σ := *)
-(*     <PC> (λ (nD' : nvmDeltaG Σ), P nD'). *)
-(* Definition post_crash_flush `{nvmFixedG Σ, nvmDeltaG Σ} *)
-(*         (P : nvmDeltaG Σ → dProp Σ) : dProp Σ := *)
+(* Definition post_crash_flush `{nvmFixedG Σ, nvmDeltaG} *)
+(*         (P : nvmDeltaG → dProp Σ) : dProp Σ := *)
+(*     <PC> (λ (nD' : nvmDeltaG), P nD'). *)
+(* Definition post_crash_flush `{nvmFixedG Σ, nvmDeltaG} *)
+(*         (P : nvmDeltaG → dProp Σ) : dProp Σ := *)
 (*   (∀ TV, monPred_in TV -∗ *)
-(*     <PC> (nD' : nvmDeltaG Σ), *)
+(*     <PC> (nD' : nvmDeltaG), *)
 (*       ∀ (CV : view), *)
 (*         ⌜ flush_view TV ⊑ CV ⌝ -∗ *)
 (*         ⎡ crashed_at CV ⎤ -∗ *)
 (*         P nD')%I. *)
 (* Next Obligation. intros ??????. apply post_crash_mono. solve_proper. Qed. *)
 
-Program Definition post_crash_flush {Σ} `{nvmFixedG Σ, nvmDeltaG Σ}
-        (P : nvmDeltaG Σ → dProp Σ) : dProp Σ :=
+Program Definition post_crash_flush {Σ} `{nvmFixedG Σ, nvmDeltaG}
+        (P : nvmDeltaG → dProp Σ) : dProp Σ :=
   MonPred (λ TV,
-    (<PC> (nD' : nvmDeltaG Σ),
+    (<PC> (nD' : nvmDeltaG),
       ∀ (CV : view),
         ⌜ flush_view TV ⊑ CV ⌝ ∗
         (* ⎡ persisted (flush_view TV) ⎤ -∗ *)
@@ -685,8 +685,8 @@ Program Definition post_crash_flush {Σ} `{nvmFixedG Σ, nvmDeltaG Σ}
 Next Obligation. intros ???????. apply post_crash_mono. solve_proper. Qed.
 
 (*
-Program Definition post_crash_flush `{hG : !nvmFixedG Σ, nvmDeltaG Σ}
-        (P : nvmFixedG Σ, nvmDeltaG Σ → dProp Σ) : dProp Σ :=
+Program Definition post_crash_flush `{hG : !nvmFixedG Σ, nvmDeltaG}
+        (P : nvmFixedG Σ, nvmDeltaG → dProp Σ) : dProp Σ :=
   MonPred (λ TV,
     (post_crash (λ hG', ∃ CV, ⌜flush_view TV ⊑ CV⌝ ∗ ⎡crashed_at CV⎤ -∗ P hG')) TV
   )%I _.
@@ -698,7 +698,7 @@ Notation "'<PCF>' g , P" :=
   (at level 200, g binder, right associativity) : bi_scope.
 
 Section post_crash_persisted.
-  Context `{hG: !nvmFixedG Σ, nvmDeltaG Σ}.
+  Context `{hG: !nvmFixedG Σ, nvmDeltaG}.
 
   Lemma post_crash_flush_post_crash P :
     post_crash P -∗
@@ -720,12 +720,12 @@ Section post_crash_persisted.
     iApply monPred_mono; done.
   Qed.
 
-  Lemma post_crash_flush_named `{nvmFixedG Σ, nvmDeltaG Σ} P name :
+  Lemma post_crash_flush_named `{nvmFixedG Σ, nvmDeltaG} P name :
     named name (post_crash_flush (λ hG, P hG)) -∗
     post_crash_flush (λ hG, named name (P hG)).
   Proof. rewrite //=. Qed.
 
-  Lemma post_crash_flush_sep `{nvmFixedG Σ, nvmDeltaG Σ} P Q :
+  Lemma post_crash_flush_sep `{nvmFixedG Σ, nvmDeltaG} P Q :
     post_crash_flush P ∗ post_crash_flush Q -∗ <PCF> hG, P hG ∗ Q hG.
   Proof.
     iStartProof (iProp _). iIntros (TV).
@@ -829,14 +829,14 @@ Section post_crash_persisted.
 
 End post_crash_persisted.
 
-Class IntoCrashFlush {Σ} `{nvmFixedG Σ, nvmDeltaG Σ}
-      (P : dProp Σ) (Q : nvmDeltaG Σ → dProp Σ) :=
+Class IntoCrashFlush {Σ} `{nvmFixedG Σ, nvmDeltaG}
+      (P : dProp Σ) (Q : nvmDeltaG → dProp Σ) :=
   into_crash_flushed : P -∗ post_crash_flush (Σ := Σ) (λ nD', Q nD').
 
 Arguments IntoCrashFlush {_} {_} {_} _%I _%I.
 
 Section IntoCrashFlush.
-  Context `{nvmFixedG Σ, nvmDeltaG Σ}.
+  Context `{nvmFixedG Σ, nvmDeltaG}.
 
   (* This is not an instance as it would probably have a negative impact on the
   performance of type class resolution. *)
@@ -940,9 +940,9 @@ Ltac iCrashFlush :=
   let H := iFresh in iIntros H; iNamed H.
 
 Section post_crash_flush_test.
-  Context `{nvmFixedG Σ, nvmDeltaG Σ}.
+  Context `{nvmFixedG Σ, nvmDeltaG}.
 
-  Lemma foo P `{Countable ST'} ℓ (ϕ : ST' → val → nvmDeltaG Σ → dProp Σ) t :
+  Lemma foo P `{Countable ST'} ℓ (ϕ : ST' → val → nvmDeltaG → dProp Σ) t :
     ⌜ P ⌝ -∗
     ⎡ know_pred ℓ ϕ ⎤ -∗
     ⎡ persisted_loc ℓ t ⎤ -∗
