src/high/modalities/fence.v
@@ -159,7 +159,7 @@ Section post_fence.
 
 End post_fence.
 
-Class IntoFenceSync `{nvmFixedG Σ, nvmDeltaG Σ}
+Class IntoFenceSync `{nvmFixedG Σ, nvmDeltaG}
       (P: dProp Σ) (Q : dProp Σ) :=
   into_fence_sync : P ⊢ <fence_sync> Q.
 Global Arguments IntoFenceSync {_} {_} {_} _%I _%I.
@@ -167,7 +167,7 @@ Global Arguments into_fence_sync {_} _%I _%I {_}.
 Global Hint Mode IntoFenceSync - - + ! -  : typeclass_instances.
 
 Section post_fence_sync.
-  Context `{nvmFixedG Σ, nvmDeltaG Σ}.
+  Context `{nvmFixedG Σ, nvmDeltaG}.
 
   Implicit Types (P : dProp Σ).
 
